
\chapter{Exercise 1}

\section{Question 1}

\subsection{Compute the expectation and the variance of this distribution}
\subsubsection{Expectation}

\begin{align}
    \begin{split}
        P(X=k) =& \; \frac{\lambda^k e^{-\lambda}}{k!} \;\; ; \; X \sim P(\lambda) \\
        E[X] =& \; \sum_{k=0}^{\infty} k \cdot P(X=k) \\
        \Rightarrow \; E[X] =& \; \sum_{k=0}^{\infty} k \cdot \frac{\lambda^k \cdot e^{-\lambda}}{k!} \\
        \Rightarrow \; E[X] =& \; \sum_{k=1}^{\infty} \frac{\lambda^{k} e^{-\lambda}}{(k-1)!} \\
        \Rightarrow \; E[X] =& \; \lambda e^{-\lambda} \cdot \sum_{k=1}^{\infty} \frac{\lambda^{k-1}}{(k-1)!} \;\; ; \;\; \lim_{n \to \infty} \sum_{n}^{\infty} \frac{\lambda^n}{n!} = e^{\lambda} \\
        \Rightarrow \; E[X] =& \; \lambda e^{-\lambda} e^{\lambda} \\
        \Rightarrow \; E[X] =& \; \lambda
    \end{split}
\end{align}

[Insert a fuckload of comments and explanations about how the Poisson Distributions' Estimator of maximum likelihood is the average, which itself is a random variable that converges towards the true value and is therefore unbiased]

\subsubsection{Variance}

\begin{align}
    \begin{split}
        P(X=k) =& \; \frac{\lambda^k e^{-\lambda}}{k!} \;\; ; \; X \sim P(\lambda) \\
        Var[X] =& \; E[X^2] - E^2[X] \\
        \Rightarrow \; Var[X] =& \; \sum_{k=0}^{\infty} k^2 \cdot P(X=k) \; - \lambda^2 \\ \\
        E[X^2] =& \sum_{k=0}^{\infty} k^2 \cdot \frac{\lambda^k \cdot e^{-\lambda}}{k!} \\
        \Rightarrow \; E[X^2] =& \; \lambda e^{-\lambda} \cdot \sum_{k=1}^{\infty} k \cdot \frac{\lambda^{k-1}}{(k-1)!} \\
        \Rightarrow \; E[X^2] =& \; \lambda e^{-\lambda} \cdot \left( \sum_{k=1}^{\infty} (k-1) \frac{\lambda^{k-1}}{(k-1)!} + \sum_{k=1}^{\infty} \frac{\lambda^{k-1}}{(k-1)!} \right) \\
        \Rightarrow \; E[X^2] =& \; \lambda e^{-\lambda} \cdot \left( \lambda \cdot \sum_{k=1}^{\infty} \frac{\lambda^{k-2}}{(k-2)!} + \sum_{k=1}^{\infty} \frac{\lambda^{k-1}}{(k-1)!} \right) \;\; ; \;\; \lim_{n \to \infty} \sum_{n}^{\infty} \frac{\lambda^n}{n!} = e^{\lambda} \\
        \Rightarrow \; E[X^2] =& \; \lambda e^{-\lambda} \cdot (\lambda e^{\lambda} + e^{\lambda}) \\
        \Rightarrow \; E[X^2] =& \; \lambda^2 + \lambda \\ \\
        \Rightarrow \; Var[X] =& \; \lambda^2 + \lambda - \lambda^2 \\
        \Rightarrow \; Var[X] =& \; \lambda
    \end{split}
\end{align}

[Insert more comments about the efficiency of the Estimator and blablabla..]